update the processor model

model/agp32ProcessorScript.sml
@@ -1,161 +1,227 @@
-open hardwarePreamble translatorTheory translatorCoreLib;
+open hardwarePreamble translatorTheory translatorCoreLib agp32StateTheory agp32EnvironmentTheory;
 
 val _ = new_theory "agp32Processor";
 
 val _ = prefer_num ();
 val _ = guess_lengths ();
 
-val _ = Datatype `
-   IF_state = <| (** fetch related **)
-                 IF_PC_input: word32;
-                 IF_PC_output: word32;
-                 IF_instr: word32;
-                 IF_PC_write_enable: bool;
-                 PC_sel: word2 
-               |>`;
+(* Pipelined Silver processor implementation *)
 
-val _ = Datatype `
-   ID_state = <| (** decode related **)
-                 ID_PC: word32;
-                 ID_instr: word32;
-                 ID_read_dataA: word32;
-                 ID_read_dataB: word32;
-                 ID_read_dataW: word32;
-                 ID_read_dataA_updated: word32;
-                 ID_read_dataB_updated: word32;
-                 ID_read_dataW_updated: word32;
-                 ID_immA: word32;
-                 ID_immB: word32;
-                 ID_immW: word32;
-                 ID_imm: word32;
-                 ID_dataA: word32;
-                 ID_dataB: word32;
-                 ID_dataW: word32;
-                 ID_ID_write_enable: bool;
-                 ID_EX_write_enable: bool;
-                 ID_flush_flag: bool;
-                 ID_addrA_enable: bool;
-                 ID_addrB_enable: bool;
-                 ID_addrW_enable: bool;
-                 ID_ForwardA: bool;
-                 ID_ForwardB: bool;
-                 ID_ForwardW: bool;
-                 ID_addrA: word6;
-                 ID_addrB: word6;
-                 ID_addrW: word6;
-                 ID_opc: word6;
-                 ID_func: word4
-               |>`;
+(* multiplexer functions used by different blocks *)
+Definition MUX_21_def:
+  MUX_21 sel input0 input1 : word32 =
+  if sel then input1 else input0
+End
 
-val _ = Datatype `
-   EX_state = <| (** execute related **)
-                 EX_PC: word32;
-                 EX_dataA: word32;
-                 EX_dataB: word32;
-                 EX_dataW: word32;
-                 EX_dataA_updated: word32;
-                 EX_dataB_updated: word32;
-                 EX_dataW_updated: word32;
-                 EX_dataA_rec: word32;
-                 EX_dataB_rec: word32;
-                 EX_dataW_rec: word32;
-                 EX_imm: word32;
-                 EX_ALU_input1: word32;
-                 EX_ALU_input2: word32;
-                 EX_ALU_res: word32;
-                 EX_SHIFT_res: word32;
-                 EX_write_enable: bool;
-                 EX_addrA_enable: bool;
-                 EX_addrB_enable: bool;
-                 EX_addrW_enable: bool;
-                 EX_isAcc: bool;
-                 EX_NOP_flag: bool;
-                 (* EX_compute_enable: bool; *)
-                 EX_PC_sel: word2;
-                 EX_ForwardA: word3;
-                 EX_ForwardB: word3;
-                 EX_ForwardW: word3;
-                 EX_addrA: word6;
-                 EX_addrB: word6;
-                 EX_addrW: word6;
-                 EX_opc: word6;
-                 EX_func: word4
-               |>`;
+Definition MUX_41_def:
+  MUX_41 (sel:word2) input0 input1 input2 input3 : word32 =
+  if sel = 0w then input0
+  else if sel = 1w then input1
+  else if sel = 2w then input2
+  else input3
+End
 
-val _ = Datatype `
-   MEM_state = <| (** memory related **)
-                 MEM_PC: word32;
-                 MEM_dataA: word32;
-                 MEM_dataB: word32;
-                 MEM_dataW: word32;
-                 MEM_imm: word32;
-                 MEM_imm_updated: word32;
-                 MEM_ALU_res: word32;
-                 MEM_SHIFT_res: word32;
-                 MEM_write_enable: bool;
-                 MEM_read_mem: bool;
-                 MEM_write_mem: bool;
-                 MEM_write_mem_byte: bool;
-                 MEM_write_reg: bool;
-                 MEM_isInterrupt: bool;
-                 MEM_state_flag: bool;
-                 MEM_NOP_flag: bool;
-                 MEM_enable: bool;
-                 MEM_addrW: word6;
-                 MEM_opc: word6 
-               |>`;
+Definition MUX_81_def:
+  MUX_81 (sel:word3) input0 input1 input2 input3 input4 input5 input6 input7 : word32 =
+  if sel = 0w then input0
+  else if sel = 1w then input1
+  else if sel = 2w then input2
+  else if sel = 3w then input3
+  else if sel = 4w then input4
+  else if sel = 5w then input5
+  else if sel = 6w then input6
+  else input7
+End
 
-val _ = Datatype `
-   WB_state = <| (** write back related **)
-                 WB_PC: word32;
-                 WB_dataA: word32;
-                 WB_read_data: word32;
-                 WB_read_data_byte: word32;
-                 WB_imm: word32;
-                 WB_ALU_res: word32;
-                 WB_SHIFT_res: word32;
-                 WB_write_data: word32;
-                 WB_write_enable: bool;
-                 WB_write_reg: bool;
-                 WB_isOut: bool;
-                 WB_state_flag: bool;
-                 WB_enable: bool;
-                 WB_data_sel: word3;
-                 WB_addrW: word6;
-                 WB_opc: word6
-               |>`;
+(* always_comb related *)
+(** compute PC **)
+Definition IF_PC_sel_update_def:
+  IF_PC_sel_update (fext:ext) (s:state_circuit) s' =
+  if (s'.EX.EX_PC_sel = 1w) \/ ((s'.EX.EX_PC_sel = 2w) /\ (s'.EX.EX_ALU_res = 0w)) \/
+     ((s'.EX.EX_PC_sel = 3w) /\ (s'.EX.EX_ALU_res <> 0w)) then
+    s' with IF := s'.IF with PC_sel := s'.EX.EX_PC_sel
+  else s' with IF := s'.IF with PC_sel := 0w  
+End
+   
+Definition IF_PC_input_update_def:
+  IF_PC_input_update (fext:ext) s s' =
+  s' with IF := s'.IF with
+                  IF_PC_input := MUX_41 s'.IF.PC_sel (s.IF.IF_PC_output + 4w) s'.EX.EX_ALU_res
+                                        (s'.EX.EX_PC + s'.EX.EX_dataW_updated)
+                                        (s'.EX.EX_PC + s'.EX.EX_dataW_updated)
+End
 
-val _ = Datatype `
-state_circuit = <|(* pipelined Silver CPU *)
+Theorem IF_PC_input_update_trans = REWRITE_RULE [MUX_41_def] IF_PC_input_update_def
 
-                 (** globel state **)
-                 state: word3;
-                 PC: word32;
-                 (* R: word6 -> word32; *)
-                 data_out: word10;
-                 data_in: word2;
-                 acc_arg: word32;
-                 acc_arg_ready: bool;
-                 interrupt_req: bool;
-                 do_interrupt: bool;
+(** get register address from instr **)
+Definition ID_addr_update_def:
+  ID_addr_update (fext:ext) (s:state_circuit) s' =
+  s' with ID := s'.ID with <| ID_addrA := (22 >< 17) s'.ID.ID_instr;
+                              ID_addrB := (15 >< 10) s'.ID.ID_instr;
+                              ID_addrW := (30 >< 25) s'.ID.ID_instr;
+                              ID_addrA_enable := word_bit 23 s'.ID.ID_instr;
+                              ID_addrB_enable := word_bit 16 s'.ID.ID_instr;
+                              ID_addrB_enable := word_bit 31 s'.ID.ID_instr
+                           |>
+End
 
-                 (** data memory interface **)
-                 command: word3;
-                 data_addr: word32;
-                 data_wdata: word32;
-                 data_wstrb: word4;
+(** decode instr **)
+Definition ID_opc_update_def:
+  ID_opc_update (fext:ext) (s:state_circuit) s' =
+  if word_bit 24 s'.ID.ID_instr then
+    if word_bit 31 s'.ID.ID_instr then
+      s' with ID := s'.ID with ID_opc := 13w
+    else if (23 >< 9) s'.ID.ID_instr = 0w then
+      s' with ID := s'.ID with ID_opc := 14w
+    else
+      s' with ID := s'.ID with ID_opc := 15w
+  else if (5 >< 0) s'.ID.ID_instr = 10w \/ (5 >< 0) s'.ID.ID_instr = 11w \/
+          (5 >< 0) s'.ID.ID_instr = 12w then                                             
+    s' with ID := s'.ID with ID_opc := (5 >< 0) s'.ID.ID_instr
+  else if word_bit 31 s'.ID.ID_instr then
+    s' with ID := s'.ID with ID_opc := 15w
+  else if (5 >< 0) s'.ID.ID_instr <+ 10w then
+    s' with ID := s'.ID with ID_opc := (5 >< 0) s'.ID.ID_instr
+  else
+    s' with ID := s'.ID with ID_opc := 15w
+End
 
-                 (** accelerator **)
-                 acc_res: word32;
-                 acc_res_ready: bool;
-                 acc_state: word2;
+Definition ID_func_update_def:
+  ID_func_update (fext:ext) (s:state_circuit) s' =
+  if s'.ID.ID_opc = 0w \/ s'.ID.ID_opc = 1w \/ s'.ID.ID_opc = 6w \/
+     s'.ID.ID_opc = 9w \/ s'.ID.ID_opc = 10w \/ s'.ID.ID_opc = 11w then
+    s' with ID := s'.ID with ID_func := (9 >< 6) s'.ID.ID_instr
+  else
+    s' with ID := s'.ID with ID_func := 9w
+End
 
-                 (** piepeline **)
-                 IF: IF_state;
-                 ID: ID_state;
-                 EX: EX_state;
-                 MEM: MEM_state;
-                 WB: WB_state 
-               |>`;
+(** register read **)
+Definition REG_read_def:
+  REG_read (fext:ext) (s:state_circuit) s' =
+  s' with ID := s'.ID with <| ID_read_dataA := s'.R s'.ID.ID_addrA;
+                              ID_read_dataB := s'.R s'.ID.ID_addrB;
+                              ID_read_dataW := s'.R s'.ID.ID_addrW 
+                           |>
+End
+
+(** generate immediate **)
+Definition ID_imm_update_def:
+  ID_imm_update (fext:ext) (s:state_circuit) s' =
+  if word_bit 31 s'.ID.ID_instr /\ word_bit 24 s'.ID.ID_instr then
+    if word_bit 23 s'.ID.ID_instr then
+      s' with ID := s'.ID with ID_imm := 0w - w2w ((22 >< 0) s'.ID.ID_instr)
+    else
+      s' with ID := s'.ID with ID_imm := w2w ((22 >< 0) s'.ID.ID_instr)
+  else if word_bit 24 s'.ID.ID_instr /\ (23 >< 9) s'.ID.ID_instr = 0w then
+    s' with ID := s'.ID with ID_imm := w2w ((8 >< 0) s'.ID.ID_instr)
+  else
+    s' with ID := s'.ID with ID_imm := 0w
+End
+
+Definition ID_imm_reg_update_def:
+  ID_imm_reg_update (fext:ext) (s:state_circuit) s' =
+  s' with ID := s'.ID with <| ID_immA := sw2sw ((22 >< 17) s'.ID.ID_instr);
+                              ID_immB := sw2sw ((15 >< 10) s'.ID.ID_instr);
+                              ID_immW := sw2sw ((30 >< 25) s'.ID.ID_instr)       
+                           |>
+End
+
+(** update the value from reg in case the addr is written by the WB stage **)
+Definition ID_foward_update_def:
+  ID_forward_update (fext:ext) (s:state_circuit) s' =
+  s' with ID := s'.ID with <| ID_ForwardA := if s'.ID.ID_addrA = s'.WB.WB_addrW /\
+                                                s'.WB.WB_write_reg /\ s'.WB.WB_state_flag then T
+                                             else F;
+                              ID_ForwardB := if s'.ID.ID_addrB = s'.WB.WB_addrW /\
+                                                s'.WB.WB_write_reg /\ s'.WB.WB_state_flag then T
+                                             else F;
+                              ID_ForwardW := if s'.ID.ID_addrW = s'.WB.WB_addrW /\
+                                                s'.WB.WB_write_reg /\ s'.WB.WB_state_flag then T
+                                             else F
+                           |>
+End
+    
+Definition ID_read_data_update_def:
+  ID_read_data_update (fext:ext) (s:state_circuit) s' =
+  s' with ID := s'.ID with <| ID_read_dataA_updated :=
+                              MUX_21 s'.ID.ID_ForwardA s'.ID.ID_read_dataA s'.WB.WB_write_data;
+                              ID_read_dataB_updated :=
+                              MUX_21 s'.ID.ID_ForwardB s'.ID.ID_read_dataB s'.WB.WB_write_data;
+                              ID_read_dataW_updated :=
+                              MUX_21 s'.ID.ID_ForwardW s'.ID.ID_read_dataW s'.WB.WB_write_data
+                           |>
+End
+
+Theorem ID_read_data_update_trans = REWRITE_RULE [MUX_21_def] ID_read_data_update_def
+
+(** update the data from read_data and imm for A/B/W **)
+Definition ID_data_update_def:
+  ID_data_update (fext:ext) (s:state_circuit) s' =
+  s' with ID := s'.ID with <| ID_dataA := MUX_21 (word_bit 23 s'.ID.ID_instr)
+                                                 s'.ID.ID_read_dataA_updated s'.ID.ID_immA;
+                              ID_dataB := MUX_21 (word_bit 16 s'.ID.ID_instr)
+                                                 s'.ID.ID_read_dataB_updated s'.ID.ID_immB;
+                              ID_dataW := MUX_21 (word_bit 31 s'.ID.ID_instr)
+                                                 s'.ID.ID_read_dataW_updated s'.ID.ID_immW
+                           |>
+End
+
+Theorem ID_data_update_trans = REWRITE_RULE [MUX_21_def] ID_data_update_def
+
+(* always_ff related: triggered by posedge clk *)
+(** Fetch: update PC **)
+Definition IF_PC_output_update_def:
+  IF_PC_output_update (fext:ext) s s' =
+  if s'.IF.IF_PC_write_enable then
+    s' with IF := s'.IF with IF_PC_output := s.IF.IF_PC_input
+  else s'
+End
+
+(** Decode: IF -> ID **)
+Definition ID_pipeline_def:
+  ID_pipeline (fext:ext) s s' =
+  if s'.ID.ID_ID_write_enable then
+    s' with ID := s'.ID with <| ID_PC := s.IF.IF_PC_output; ID_instr := s.IF.IF_instr |>
+  else if s'.ID.ID_flush_flag then
+    s' with ID := s'.ID with ID_instr := 0x0000003Fw
+  else s'
+End
+
+(** register write **)
+Definition REG_write_def:
+  REG_write (fext:ext) (s:state_circuit) s' =
+  if s'.WB.WB_write_reg /\ s'.WB.WB_state_flag then
+    s' with R := (s'.WB.WB_addrW =+ s'.WB.WB_write_data) s'.R
+  else s'
+End
+
+(* processor *)
+val init_tm = add_x_inits “<|PC := 0w;
+                             R := K 0w;
+                             state := 3w;
+                             acc_arg_ready := F;
+                             command := 0w;
+                             do_interrupt := F;
+                             interrupt_req := F;
+                             IF := <| IF_PC_output := 0w |>;
+                             ID := <| ID_instr := 0x0000003Fw; ID_ForwardA := F; ID_ForwardB := F;
+                                      ID_ForwardW := F
+                                   |>;
+                             EX := <| EX_PC := 0w |>;
+                             MEM := <| MEM_PC := 0w |>;
+                             WB := <| WB_PC := 0w |> |>”;
+
+Definition agp32_init_def:
+  agp32_init fbits = ^init_tm
+End
+
+Definition agp32_def:
+  agp32 = mk_module (procs [IF_PC_output_update; ID_pipeline; REG_write])
+                    (procs [IF_PC_sel_update; IF_PC_input_update; ID_addr_update;
+                            ID_opc_update; ID_func_update; REG_read; ID_imm_update;
+                            ID_imm_reg_update; ID_forward_update; ID_read_data_update;
+                            ID_data_update])
+                    agp32_init
+End
 
 val _ = export_theory ();
