model/compilation/agp32VerilogScript.sml
@@ -1,0 +1,31 @@
+open hardwarePreamble alignmentTheory alistTheory agp32StateTheory agp32ProcessorTheory translatorLib verilogPrintLib;
+
+val _ = new_theory "agp32Verilog";
+
+val _ = guess_lengths ();
+val _ = prefer_num ();
+
+val module_def = agp32_def;
+val abstract_fields = ["mem", "io_events", "interrupt_state"];
+val outputs = ["PC"];
+val comms = ["PC", "data_out",
+             "command", "data_addr", "data_wdata", "data_wstrb",
+             "acc_arg", "acc_arg_ready",
+             "acc_res", "acc_res_ready",
+             "interrupt_req"];
+
+val trans_thm = module2hardware module_def
+                                abstract_fields
+                                outputs
+                                comms;
+
+val verilogstr =
+ definition"agp32_v_def"
+ |> REWRITE_RULE [definition"agp32_v_seqs_def", definition"agp32_v_combs_def"]
+ |> concl
+ |> rhs
+ |> verilog_print "agp32_processor";
+
+val _ = writeFile "agp32_processor.sv" verilogstr;
+
+val _ = export_theory ();
